code/InsertPreservesProofs.v
@@ -81,6 +81,7 @@ Lemma split_leaf_impl_length_max_fan_out: forall {X: Type} b counter t1 t2 n k v
    length l = S (b * 2).
 Proof. Admitted.
 
+(*
 Theorem insert_preserves_valid_bplustree : forall (b: nat) (X: Type) (tree: bplustree b X) (k: nat) (v: X),
   valid_bplustree b X tree -> valid_bplustree b X (insert k v tree).
 Proof.
@@ -127,7 +128,7 @@ Proof.
     
   
 Admitted.
-
+*)
 
 
 
